More operations

pulse/examples/steel/Selectors.Tree.fsti
@@ -16,7 +16,7 @@ let t (a: Type0) = ref (node a)
 (** This type reflects the contents of a tree without the memory layout *)
 type tree (a: Type0) =
   | Leaf : tree a
-  | Node: left: a -> right: a -> tree a
+  | Node: data: a -> left: tree a -> right: tree a -> tree a
 
 (**** Slprop and selector *)
 
@@ -54,13 +54,13 @@ let v_linked_tree
 
 val get_left (#a: Type0) (n: node a) : t a
 val get_right (#a: Type0) (n: node a) : t a
-val data (#a: Type0) (n: node a) : a
+val get_data (#a: Type0) (n: node a) : a
 val mk_node (#a: Type0) (left right: t a) (v: a)
     : Pure (node a)
       (requires True)
-      (ensures (fun n -> get_left n == left /\ get_right n == right /\ data n == v))
+      (ensures (fun n -> get_left n == left /\ get_right n == right /\ get_data n == v))
 
-(**** Operations on lists *)
+(**** Low-level operations on trees *)
 
 val null_t (#a: Type0) : t a
 val is_null_t (#a: Type0) (r: t a) : (b:bool{b <==> r == null_t})
@@ -78,3 +78,44 @@ val elim_linked_tree_leaf (#a: Type0) (ptr: t a)
        (ensures (fun h0 _ h1 ->
          v_linked_tree ptr h0 == v_linked_tree ptr h1 /\
          v_linked_tree ptr h1 == Leaf))
+
+val update_data (#a: Type0) (ptr: t a) (new_v: a)
+    : SteelSel unit
+      (linked_tree ptr) (fun _ -> linked_tree ptr)
+      (requires (fun h0 -> Node? (v_linked_tree ptr h0) /\ not (is_null_t ptr)))
+      (ensures (fun h0 _ h1 ->
+        Node? (v_linked_tree ptr h0) /\ ( // For AF: do not repeat precondition?
+        let Node old_v left right = v_linked_tree ptr h0 in
+        v_linked_tree ptr h1 == Node new_v left right
+      )))
+
+val intro_tree_left_cons (#a: Type0) (ptr: t a) (left : t a)
+    : SteelSel unit
+      (vptr ptr `star` linked_tree left)
+      (fun _ ->  vptr ptr `star` linked_tree left)
+      (requires (fun h0 -> get_left (sel ptr h0) == null_t))
+      (ensures (fun h0 _ h1 ->
+        get_data (sel ptr h1) == get_data (sel ptr h0) /\
+        get_left (sel ptr h1) == left /\
+        get_right (sel ptr h1) == get_right (sel ptr h0) /\
+        v_linked_tree left h0 == v_linked_tree left h1
+      ))
+
+
+(**** High-level operations on trees *)
+
+val append_tree_left (#a: Type0) (ptr: t a) (left : t a)
+    : SteelSel unit
+      (linked_tree ptr `star` linked_tree left)
+      (fun _ ->  linked_tree ptr)
+      (requires (fun h0 -> match v_linked_tree ptr h0 with Node _ Leaf _ -> True | _ -> False))
+      (ensures (fun h0 _ h1 ->
+        match v_linked_tree ptr h0, v_linked_tree ptr h1 with
+        | Node old_data Leaf old_right, Node new_data new_left new_right ->
+          old_data == new_data /\
+          new_left == v_linked_tree left h0 /\
+          new_right == old_right
+        | _, _ -> False
+      ))
+
+(** Self-balancing part of trees *)
